@prefix : <http://www.w3id.org/arco/ontology/content#> .
@prefix owl: <http://www.w3.org/2002/07/owl#> .
@prefix rdf: <http://www.w3.org/1999/02/22-rdf-syntax-ns#> .
@prefix xml: <http://www.w3.org/XML/1998/namespace> .
@prefix xsd: <http://www.w3.org/2001/XMLSchema#> .
@prefix rdfs: <http://www.w3.org/2000/01/rdf-schema#> .
@base <http://www.w3id.org/arco/ontology/content> .

<http://www.w3id.org/arco/ontology/content> rdf:type owl:Ontology ;
                                             owl:imports <https://w3id.org/arco/ontology/context-description> ,
                                                         <https://w3id.org/arco/ontology/denotative-description> .

#################################################################
#    Object Properties
#################################################################

###  http://www.w3id.org/arco/ontology/content/defines
<http://www.w3id.org/arco/ontology/content/defines> rdf:type owl:ObjectProperty ;
                                                    rdfs:comment "This property define the act of attaching a meaning to a term."@en .


###  http://www.w3id.org/arco/ontology/content/hasAuthor
<http://www.w3id.org/arco/ontology/content/hasAuthor> rdf:type owl:ObjectProperty ;
                                                      owl:inverseOf <http://www.w3id.org/arco/ontology/content/isAuthorOf> ;
                                                      rdfs:comment "This property links any written work to its creator or originator."@en .


###  http://www.w3id.org/arco/ontology/content/hasBusinessPartner
<http://www.w3id.org/arco/ontology/content/hasBusinessPartner> rdf:type owl:ObjectProperty ;
                                                               rdfs:subPropertyOf <http://www.w3id.org/arco/ontology/content/isRelatedTo> ;
                                                               rdf:type owl:SymmetricProperty ;
                                                               rdfs:comment "This property defines a business relations bwtween two agents."@en .


###  http://www.w3id.org/arco/ontology/content/hasCharacter
<http://www.w3id.org/arco/ontology/content/hasCharacter> rdf:type owl:ObjectProperty ;
                                                         owl:inverseOf <http://www.w3id.org/arco/ontology/content/isCharacterOf> .


###  http://www.w3id.org/arco/ontology/content/hasCharacterRole
<http://www.w3id.org/arco/ontology/content/hasCharacterRole> rdf:type owl:ObjectProperty ;
                                                             rdfs:subPropertyOf <http://www.w3id.org/arco/ontology/content/hasType> ;
                                                             owl:inverseOf <http://www.w3id.org/arco/ontology/content/isCharacterRole> ;
                                                             rdfs:comment "This property defines character’s role as protagonist, antagonist or secondary."@en .


###  http://www.w3id.org/arco/ontology/content/hasCharacterScope
<http://www.w3id.org/arco/ontology/content/hasCharacterScope> rdf:type owl:ObjectProperty ;
                                                              rdfs:subPropertyOf <http://www.w3id.org/arco/ontology/content/hasType> ;
                                                              owl:inverseOf <http://www.w3id.org/arco/ontology/content/isCharacterScope> ;
                                                              rdfs:comment "This property defines character’s scope as universal good, universal bad or self good."@en .


###  http://www.w3id.org/arco/ontology/content/hasCharacterStatus
<http://www.w3id.org/arco/ontology/content/hasCharacterStatus> rdf:type owl:ObjectProperty ;
                                                               rdfs:subPropertyOf <http://www.w3id.org/arco/ontology/content/hasType> ;
                                                               owl:inverseOf <http://www.w3id.org/arco/ontology/content/isCharacterStatus> ;
                                                               rdfs:comment "This property defines character’s status as leading, opposing or supporting."@en .


###  http://www.w3id.org/arco/ontology/content/hasCharacterType
<http://www.w3id.org/arco/ontology/content/hasCharacterType> rdf:type owl:ObjectProperty ;
                                                             rdfs:subPropertyOf <http://www.w3id.org/arco/ontology/content/hasType> ;
                                                             owl:inverseOf <http://www.w3id.org/arco/ontology/content/isCharacterType> ;
                                                             rdfs:comment "This property defines character’s type as hero, antihero, or villain."@en .


###  http://www.w3id.org/arco/ontology/content/hasChild
<http://www.w3id.org/arco/ontology/content/hasChild> rdf:type owl:ObjectProperty ;
                                                     rdfs:subPropertyOf <http://www.w3id.org/arco/ontology/content/hasRelative> ;
                                                     owl:inverseOf <http://www.w3id.org/arco/ontology/content/hasParent> ;
                                                     rdfs:comment "This property links an agent that is parent to another agent."@en .


###  http://www.w3id.org/arco/ontology/content/hasEmployee
<http://www.w3id.org/arco/ontology/content/hasEmployee> rdf:type owl:ObjectProperty ;
                                                        rdfs:subPropertyOf <http://www.w3id.org/arco/ontology/content/isRelatedTo> ;
                                                        owl:inverseOf <http://www.w3id.org/arco/ontology/content/hasEmployer> ;
                                                        rdfs:comment "This property links an employer to its employee."@en .


###  http://www.w3id.org/arco/ontology/content/hasEmployer
<http://www.w3id.org/arco/ontology/content/hasEmployer> rdf:type owl:ObjectProperty ;
                                                        rdfs:subPropertyOf <http://www.w3id.org/arco/ontology/content/isRelatedTo> ;
                                                        rdfs:comment "This property links an employee to its employer."@en .


###  http://www.w3id.org/arco/ontology/content/hasEnvironment
<http://www.w3id.org/arco/ontology/content/hasEnvironment> rdf:type owl:ObjectProperty ;
                                                           rdfs:subPropertyOf <http://www.w3id.org/arco/ontology/content/hasSociologicalCharacteristic> ;
                                                           rdfs:comment "This property links an agent to an environment."@en .


###  http://www.w3id.org/arco/ontology/content/hasEthnicGroup
<http://www.w3id.org/arco/ontology/content/hasEthnicGroup> rdf:type owl:ObjectProperty ;
                                                           rdfs:subPropertyOf <http://www.w3id.org/arco/ontology/content/hasSociologicalCharacteristic> ;
                                                           owl:inverseOf <http://www.w3id.org/arco/ontology/content/isEthnicGroupOf> ;
                                                           rdfs:comment "This property links an agent to an ethnic group."@en .


###  http://www.w3id.org/arco/ontology/content/hasEthnicOrigin
<http://www.w3id.org/arco/ontology/content/hasEthnicOrigin> rdf:type owl:ObjectProperty ;
                                                            rdfs:subPropertyOf <http://www.w3id.org/arco/ontology/content/hasOrigin> ;
                                                            owl:inverseOf <http://www.w3id.org/arco/ontology/content/isEthnicOriginOf> ;
                                                            rdfs:comment "This property defines the origin an agent has from an ethnic point of view."@en .


###  http://www.w3id.org/arco/ontology/content/hasFictionalType
<http://www.w3id.org/arco/ontology/content/hasFictionalType> rdf:type owl:ObjectProperty ;
                                                             rdfs:subPropertyOf <http://www.w3id.org/arco/ontology/content/hasType> ;
                                                             owl:inverseOf <http://www.w3id.org/arco/ontology/content/isFictionalType> ;
                                                             rdfs:comment "This property defines fictional character’s type as fictional or non fictional."@en .


###  http://www.w3id.org/arco/ontology/content/hasGeographicOrigin
<http://www.w3id.org/arco/ontology/content/hasGeographicOrigin> rdf:type owl:ObjectProperty ;
                                                                rdfs:subPropertyOf <http://www.w3id.org/arco/ontology/content/hasOrigin> ;
                                                                owl:inverseOf <http://www.w3id.org/arco/ontology/content/isGeographicOriginOf> ;
                                                                rdfs:comment "This property defines the origin an agent has from a geographic point of view."@en .


###  http://www.w3id.org/arco/ontology/content/hasOrigin
<http://www.w3id.org/arco/ontology/content/hasOrigin> rdf:type owl:ObjectProperty ;
                                                      rdfs:subPropertyOf <http://www.w3id.org/arco/ontology/content/hasSociologicalCharacteristic> ;
                                                      rdfs:comment "This property defines the origin an agent has."@en .


###  http://www.w3id.org/arco/ontology/content/hasParent
<http://www.w3id.org/arco/ontology/content/hasParent> rdf:type owl:ObjectProperty ;
                                                      rdfs:subPropertyOf <http://www.w3id.org/arco/ontology/content/hasRelative> ;
                                                      rdfs:comment "This property link an agent that is child to another agent."@en .


###  http://www.w3id.org/arco/ontology/content/hasPartIn
<http://www.w3id.org/arco/ontology/content/hasPartIn> rdf:type owl:ObjectProperty ;
                                                      rdfs:comment "To be involved in, to be a factor in."@en .


###  http://www.w3id.org/arco/ontology/content/hasProfession
<http://www.w3id.org/arco/ontology/content/hasProfession> rdf:type owl:ObjectProperty ;
                                                          rdfs:subPropertyOf <http://www.w3id.org/arco/ontology/content/hasSociologicalCharacteristic> ;
                                                          rdfs:comment "This property links an agent to a profession."@en .


###  http://www.w3id.org/arco/ontology/content/hasRelative
<http://www.w3id.org/arco/ontology/content/hasRelative> rdf:type owl:ObjectProperty ;
                                                        rdfs:subPropertyOf <http://www.w3id.org/arco/ontology/content/isRelatedTo> ;
                                                        rdf:type owl:SymmetricProperty ;
                                                        rdfs:comment "This property links two agents connected by blood or marriage."@en .


###  http://www.w3id.org/arco/ontology/content/hasRole
<http://www.w3id.org/arco/ontology/content/hasRole> rdf:type owl:ObjectProperty ;
                                                    owl:inverseOf <http://www.w3id.org/arco/ontology/content/isRole> ;
                                                    rdfs:comment "This property defines the role of character in a play."@en .


###  http://www.w3id.org/arco/ontology/content/hasSocialOrigin
<http://www.w3id.org/arco/ontology/content/hasSocialOrigin> rdf:type owl:ObjectProperty ;
                                                            rdfs:subPropertyOf <http://www.w3id.org/arco/ontology/content/hasOrigin> ;
                                                            rdf:type owl:FunctionalProperty ;
                                                            rdfs:comment "This property defines the origin an agent has from a social point of view."@en .


###  http://www.w3id.org/arco/ontology/content/hasSociologicalCharacteristic
<http://www.w3id.org/arco/ontology/content/hasSociologicalCharacteristic> rdf:type owl:ObjectProperty ;
                                                                          owl:inverseOf <http://www.w3id.org/arco/ontology/content/isSociologicalCharacteristicOf> ;
                                                                          rdfs:comment "This property defines a sociological characteristic that can be described as belonging to an agent."@en .


###  http://www.w3id.org/arco/ontology/content/hasSpinOff
<http://www.w3id.org/arco/ontology/content/hasSpinOff> rdf:type owl:ObjectProperty ;
                                                       owl:inverseOf <http://www.w3id.org/arco/ontology/content/isSpinOffOf> ;
                                                       rdfs:comment "This property links a TV serie to another TV serie in which a secondary character in the first show becomes the protagonist."@en .


###  http://www.w3id.org/arco/ontology/content/hasType
<http://www.w3id.org/arco/ontology/content/hasType> rdf:type owl:ObjectProperty ;
                                                    owl:inverseOf <http://www.w3id.org/arco/ontology/content/isType> ;
                                                    rdfs:comment "This property defines the typology of character depicted as human, animal or supernatural one."@en .


###  http://www.w3id.org/arco/ontology/content/isAuthorOf
<http://www.w3id.org/arco/ontology/content/isAuthorOf> rdf:type owl:ObjectProperty ;
                                                       rdfs:comment "This property links a creator or originator to its written work."@en .


###  http://www.w3id.org/arco/ontology/content/isBasedOn
<http://www.w3id.org/arco/ontology/content/isBasedOn> rdf:type owl:ObjectProperty ,
                                                               owl:FunctionalProperty ,
                                                               owl:InverseFunctionalProperty ;
                                                      rdfs:comment "This property defines a character that is based on or inspired to a real or invented person, animal or supernatural being."@en .


###  http://www.w3id.org/arco/ontology/content/isCharacterOf
<http://www.w3id.org/arco/ontology/content/isCharacterOf> rdf:type owl:ObjectProperty .


###  http://www.w3id.org/arco/ontology/content/isCharacterRole
<http://www.w3id.org/arco/ontology/content/isCharacterRole> rdf:type owl:ObjectProperty ;
                                                            rdfs:subPropertyOf <http://www.w3id.org/arco/ontology/content/isType> ;
                                                            rdfs:comment "This property defines protagonist, antagonist and secondary as character’s role."@en .


###  http://www.w3id.org/arco/ontology/content/isCharacterScope
<http://www.w3id.org/arco/ontology/content/isCharacterScope> rdf:type owl:ObjectProperty ;
                                                             rdfs:subPropertyOf <http://www.w3id.org/arco/ontology/content/isType> ;
                                                             rdfs:comment "This property defines universal good, universal bad and self good as character’s scope."@en .


###  http://www.w3id.org/arco/ontology/content/isCharacterStatus
<http://www.w3id.org/arco/ontology/content/isCharacterStatus> rdf:type owl:ObjectProperty ;
                                                              rdfs:subPropertyOf <http://www.w3id.org/arco/ontology/content/isType> ;
                                                              rdfs:comment "This property defines leading, opposing, and supporting as character’s status."@en .


###  http://www.w3id.org/arco/ontology/content/isCharacterType
<http://www.w3id.org/arco/ontology/content/isCharacterType> rdf:type owl:ObjectProperty ;
                                                            rdfs:subPropertyOf <http://www.w3id.org/arco/ontology/content/isType> ;
                                                            rdfs:comment "This property defines hero, antihero, and villain as character’s type."@en .


###  http://www.w3id.org/arco/ontology/content/isDefinedBy
<http://www.w3id.org/arco/ontology/content/isDefinedBy> rdf:type owl:ObjectProperty ;
                                                        rdfs:comment "This property defines the meaning that is attached to a term."@en .


###  http://www.w3id.org/arco/ontology/content/isEnvironmentOf
<http://www.w3id.org/arco/ontology/content/isEnvironmentOf> rdf:type owl:ObjectProperty ;
                                                            rdfs:subPropertyOf <http://www.w3id.org/arco/ontology/content/isSociologicalCharacteristicOf> ;
                                                            rdfs:comment "This property links an environment to an agent."@en .


###  http://www.w3id.org/arco/ontology/content/isEthnicGroupOf
<http://www.w3id.org/arco/ontology/content/isEthnicGroupOf> rdf:type owl:ObjectProperty ;
                                                            rdfs:subPropertyOf <http://www.w3id.org/arco/ontology/content/isSociologicalCharacteristicOf> ;
                                                            rdfs:comment "This property links an ethnic group to an agent."@en .


###  http://www.w3id.org/arco/ontology/content/isEthnicOriginOf
<http://www.w3id.org/arco/ontology/content/isEthnicOriginOf> rdf:type owl:ObjectProperty ;
                                                             rdfs:subPropertyOf <http://www.w3id.org/arco/ontology/content/isOriginOf> ;
                                                             rdfs:comment "This property defines the origin referring to an agent from an ethnic point of view."@en .


###  http://www.w3id.org/arco/ontology/content/isFictionalType
<http://www.w3id.org/arco/ontology/content/isFictionalType> rdf:type owl:ObjectProperty ;
                                                            rdfs:subPropertyOf <http://www.w3id.org/arco/ontology/content/isType> ;
                                                            rdfs:comment "This property defines fictional and non fictional as character’s fictional type."@en .


###  http://www.w3id.org/arco/ontology/content/isGeographicOriginOf
<http://www.w3id.org/arco/ontology/content/isGeographicOriginOf> rdf:type owl:ObjectProperty ;
                                                                 rdfs:subPropertyOf <http://www.w3id.org/arco/ontology/content/isOriginOf> ;
                                                                 rdfs:comment "This property defines the origin referring to an agent from a geographic point of view."@en .


###  http://www.w3id.org/arco/ontology/content/isKilledBy
<http://www.w3id.org/arco/ontology/content/isKilledBy> rdf:type owl:ObjectProperty ;
                                                       owl:inverseOf <http://www.w3id.org/arco/ontology/content/kills> ;
                                                       rdfs:comment "This property links two agents in which the first one is killed by the second one."@en .


###  http://www.w3id.org/arco/ontology/content/isOriginOf
<http://www.w3id.org/arco/ontology/content/isOriginOf> rdf:type owl:ObjectProperty ;
                                                       rdfs:subPropertyOf <http://www.w3id.org/arco/ontology/content/isSociologicalCharacteristicOf> ;
                                                       rdfs:comment "This property defines the origin referring to an agent."@en .


###  http://www.w3id.org/arco/ontology/content/isPlayedBy
<http://www.w3id.org/arco/ontology/content/isPlayedBy> rdf:type owl:ObjectProperty ;
                                                       owl:inverseOf <http://www.w3id.org/arco/ontology/content/plays> ;
                                                       rdfs:comment "This property defines a character that is interpreted by an actor."@en .


###  http://www.w3id.org/arco/ontology/content/isProfessionOf
<http://www.w3id.org/arco/ontology/content/isProfessionOf> rdf:type owl:ObjectProperty ;
                                                           rdfs:subPropertyOf <http://www.w3id.org/arco/ontology/content/isSociologicalCharacteristicOf> ;
                                                           rdfs:comment "This property link a profession to an agent."@en .


###  http://www.w3id.org/arco/ontology/content/isRelatedTo
<http://www.w3id.org/arco/ontology/content/isRelatedTo> rdf:type owl:ObjectProperty ,
                                                                 owl:SymmetricProperty ;
                                                        rdfs:comment "This property defines a personal relations between two agents."@en .


###  http://www.w3id.org/arco/ontology/content/isRole
<http://www.w3id.org/arco/ontology/content/isRole> rdf:type owl:ObjectProperty ;
                                                   rdfs:comment "This property defines a character by its role in a play."@en .


###  http://www.w3id.org/arco/ontology/content/isSocialOriginOf
<http://www.w3id.org/arco/ontology/content/isSocialOriginOf> rdf:type owl:ObjectProperty ;
                                                             rdfs:subPropertyOf <http://www.w3id.org/arco/ontology/content/isOriginOf> ;
                                                             rdfs:comment "This property defines the origin referring to an agent from a social point of view."@en .


###  http://www.w3id.org/arco/ontology/content/isSociologicalCharacteristicOf
<http://www.w3id.org/arco/ontology/content/isSociologicalCharacteristicOf> rdf:type owl:ObjectProperty ;
                                                                           rdfs:comment "This property defines a sociological characteristic that refers to an agent." .


###  http://www.w3id.org/arco/ontology/content/isSpinOffOf
<http://www.w3id.org/arco/ontology/content/isSpinOffOf> rdf:type owl:ObjectProperty ;
                                                        rdfs:comment "This property links a TV serie to another TV serie in which the protagonist played a secondary role."@en .


###  http://www.w3id.org/arco/ontology/content/isType
<http://www.w3id.org/arco/ontology/content/isType> rdf:type owl:ObjectProperty ;
                                                   rdfs:comment "This property defines human, animal or supernatural being as typology of character."@en .


###  http://www.w3id.org/arco/ontology/content/kills
<http://www.w3id.org/arco/ontology/content/kills> rdf:type owl:ObjectProperty ;
                                                  rdfs:comment "This property links two agents in which the first one kills the second one."@en .


###  http://www.w3id.org/arco/ontology/content/plays
<http://www.w3id.org/arco/ontology/content/plays> rdf:type owl:ObjectProperty ;
                                                  rdfs:comment "This property defines an actor that interprets a character."@en .


###  https://w3id.org/arco/ontology/denotative-description/basedOn
<https://w3id.org/arco/ontology/denotative-description/basedOn> rdf:type owl:ObjectProperty ;
                                                                rdfs:comment "The relation that links the subject, that is the scenario, to a cultural property."@en .


###  https://w3id.org/arco/ontology/denotative-description/includes
<https://w3id.org/arco/ontology/denotative-description/includes> rdf:type owl:ObjectProperty ;
                                                                 rdfs:comment "The relation that links the subject, that is the scenario, to a cultural property."@en .


###  https://w3id.org/arco/ontology/denotative-description/isIncludedIn
<https://w3id.org/arco/ontology/denotative-description/isIncludedIn> rdf:type owl:ObjectProperty ;
                                                                     rdfs:comment "The relation that connects the plot to the scenario."@en .


#################################################################
#    Data properties
#################################################################

###  http://www.w3id.org/arco/ontology/content/hasAlternativeName
<http://www.w3id.org/arco/ontology/content/hasAlternativeName> rdf:type owl:DatatypeProperty ;
                                                               rdfs:subPropertyOf <http://www.w3id.org/arco/ontology/content/hasName> ;
                                                               rdfs:range xsd:string .


###  http://www.w3id.org/arco/ontology/content/hasBirthDate
<http://www.w3id.org/arco/ontology/content/hasBirthDate> rdf:type owl:DatatypeProperty ;
                                                         rdfs:range xsd:dateTime ;
                                                         rdfs:comment "This property associates an agent to the day of its birth."@en .


###  http://www.w3id.org/arco/ontology/content/hasDeathDate
<http://www.w3id.org/arco/ontology/content/hasDeathDate> rdf:type owl:DatatypeProperty ;
                                                         rdfs:range xsd:dateTime ;
                                                         rdfs:comment "This property associates an agent to the day of its death."@en .


###  http://www.w3id.org/arco/ontology/content/hasFirstName
<http://www.w3id.org/arco/ontology/content/hasFirstName> rdf:type owl:DatatypeProperty ;
                                                         rdfs:subPropertyOf <http://www.w3id.org/arco/ontology/content/hasName> ;
                                                         rdfs:comment "This property links an agent to its first name."@en .


###  http://www.w3id.org/arco/ontology/content/hasLastName
<http://www.w3id.org/arco/ontology/content/hasLastName> rdf:type owl:DatatypeProperty ;
                                                        rdfs:subPropertyOf <http://www.w3id.org/arco/ontology/content/hasName> ;
                                                        rdfs:comment "This property links an agent to its last name."@en .


###  http://www.w3id.org/arco/ontology/content/hasName
<http://www.w3id.org/arco/ontology/content/hasName> rdf:type owl:DatatypeProperty ;
                                                    rdfs:range xsd:string ;
                                                    rdfs:comment "This property links an agent to its name."@en .


###  http://www.w3id.org/arco/ontology/content/hasNickname
<http://www.w3id.org/arco/ontology/content/hasNickname> rdf:type owl:DatatypeProperty ;
                                                        rdfs:subPropertyOf <http://www.w3id.org/arco/ontology/content/hasAlternativeName> ;
                                                        rdfs:range xsd:string ;
                                                        rdfs:comment "This property links an agent to its nickname."@en .


###  http://www.w3id.org/arco/ontology/content/hasPlaceOfBirth
<http://www.w3id.org/arco/ontology/content/hasPlaceOfBirth> rdf:type owl:DatatypeProperty ;
                                                            rdfs:comment "This property links an agent to the geografical place in which it was born."@en .


###  http://www.w3id.org/arco/ontology/content/hasPlaceOfDeath
<http://www.w3id.org/arco/ontology/content/hasPlaceOfDeath> rdf:type owl:DatatypeProperty ;
                                                            rdfs:comment "This property links an agent to the geografical place in which it died."@en .


###  http://www.w3id.org/arco/ontology/content/hasPlaceOfLiving
<http://www.w3id.org/arco/ontology/content/hasPlaceOfLiving> rdf:type owl:DatatypeProperty ;
                                                             rdfs:comment "This property links an agent to the geografical place in which it lives."@en .


###  http://www.w3id.org/arco/ontology/content/hasPseudonym
<http://www.w3id.org/arco/ontology/content/hasPseudonym> rdf:type owl:DatatypeProperty ;
                                                         rdfs:subPropertyOf <http://www.w3id.org/arco/ontology/content/hasAlternativeName> ;
                                                         rdfs:range xsd:string ;
                                                         rdfs:comment "This property links an agent to its pseudonym."@en .


###  http://www.w3id.org/arco/ontology/content/hasSex
<http://www.w3id.org/arco/ontology/content/hasSex> rdf:type owl:DatatypeProperty ;
                                                   rdfs:range xsd:string ;
                                                   rdfs:comment "This property links an agent to its biological sex."@en .


#################################################################
#    Classes
#################################################################

###  http://dati.beniculturali.it/cis/CulturalEntity
<http://dati.beniculturali.it/cis/CulturalEntity> owl:equivalentClass <http://www.w3id.org/arco/ontology/content/CulturalProduct> .


###  http://dati.gov.it/onto/dcatapit#Agent
<http://dati.gov.it/onto/dcatapit#Agent> owl:equivalentClass <http://www.w3id.org/arco/ontology/content/Agent> .


###  http://www.w3id.org/arco/ontology/content/Actor
<http://www.w3id.org/arco/ontology/content/Actor> rdf:type owl:Class ;
                                                  rdfs:subClassOf <http://www.w3id.org/arco/ontology/content/Person> ;
                                                  rdfs:comment "This class refers to a person who’s profession is acting on stage, films, or television."@en .


###  http://www.w3id.org/arco/ontology/content/Agent
<http://www.w3id.org/arco/ontology/content/Agent> rdf:type owl:Class ;
                                                  owl:equivalentClass <https://w3id.org/italia/onto/l0/Agent> ;
                                                  rdfs:subClassOf owl:Thing ,
                                                                  [ rdf:type owl:Restriction ;
                                                                    owl:onProperty <http://www.w3id.org/arco/ontology/content/hasProfession> ;
                                                                    owl:someValuesFrom <http://www.w3id.org/arco/ontology/content/Profession>
                                                                  ] ,
                                                                  [ rdf:type owl:Restriction ;
                                                                    owl:onProperty <http://www.w3id.org/arco/ontology/content/hasSocialOrigin> ;
                                                                    owl:maxQualifiedCardinality "1"^^xsd:nonNegativeInteger ;
                                                                    owl:onClass <http://www.w3id.org/arco/ontology/content/SocialOrigin>
                                                                  ] ;
                                                  owl:disjointWith <http://www.w3id.org/arco/ontology/content/SociologicalCharacteristics> .


###  http://www.w3id.org/arco/ontology/content/Animal
<http://www.w3id.org/arco/ontology/content/Animal> rdf:type owl:Class ;
                                                   rdfs:subClassOf <http://www.w3id.org/arco/ontology/content/Agent> ;
                                                   rdfs:comment "This class refers to living organism that feeds on organic matter."@en .


###  http://www.w3id.org/arco/ontology/content/Antagonist
<http://www.w3id.org/arco/ontology/content/Antagonist> rdf:type owl:Class ;
                                                       rdfs:subClassOf <http://www.w3id.org/arco/ontology/content/CharacterRole> ,
                                                                       [ rdf:type owl:Restriction ;
                                                                         owl:onProperty <http://www.w3id.org/arco/ontology/content/hasCharacterStatus> ;
                                                                         owl:allValuesFrom <http://www.w3id.org/arco/ontology/content/Opposing>
                                                                       ] ;
                                                       rdfs:comment "This class refers to a character of a work actively opposing the protagonist."@en .


###  http://www.w3id.org/arco/ontology/content/AntiHero
<http://www.w3id.org/arco/ontology/content/AntiHero> rdf:type owl:Class ;
                                                     rdfs:subClassOf <http://www.w3id.org/arco/ontology/content/CharacterType> ,
                                                                     [ rdf:type owl:Restriction ;
                                                                       owl:onProperty <http://www.w3id.org/arco/ontology/content/hasCharacterStatus> ;
                                                                       owl:someValuesFrom <http://www.w3id.org/arco/ontology/content/CharacterStatus>
                                                                     ] ,
                                                                     [ rdf:type owl:Restriction ;
                                                                       owl:onProperty <http://www.w3id.org/arco/ontology/content/hasCharacterRole> ;
                                                                       owl:allValuesFrom [ rdf:type owl:Class ;
                                                                                           owl:unionOf ( <http://www.w3id.org/arco/ontology/content/Antagonist>
                                                                                                         <http://www.w3id.org/arco/ontology/content/CharacterStatus>
                                                                                                         <http://www.w3id.org/arco/ontology/content/Protagonist>
                                                                                                         <http://www.w3id.org/arco/ontology/content/Secondary>
                                                                                                       )
                                                                                         ]
                                                                     ] ,
                                                                     [ rdf:type owl:Restriction ;
                                                                       owl:onProperty <http://www.w3id.org/arco/ontology/content/hasCharacterScope> ;
                                                                       owl:allValuesFrom <http://www.w3id.org/arco/ontology/content/SelfGood>
                                                                     ] ;
                                                     rdfs:comment "This class refers to a leading character in a film, book or play, who is devoid of heroic qualities."@en .


###  http://www.w3id.org/arco/ontology/content/Aristocracy
<http://www.w3id.org/arco/ontology/content/Aristocracy> rdf:type owl:Class ;
                                                        rdfs:subClassOf <http://www.w3id.org/arco/ontology/content/SocialClass> ;
                                                        owl:disjointWith <http://www.w3id.org/arco/ontology/content/Clergy> ,
                                                                         <http://www.w3id.org/arco/ontology/content/Commoner> ;
                                                        rdfs:comment "This class refers to the social class aristocrats are recognized to belong to."@en .


###  http://www.w3id.org/arco/ontology/content/Author
<http://www.w3id.org/arco/ontology/content/Author> rdf:type owl:Class ;
                                                   rdfs:subClassOf <http://www.w3id.org/arco/ontology/content/Writer> ;
                                                   rdfs:comment "This class refers to a writer of any written work."@en .


###  http://www.w3id.org/arco/ontology/content/Character
<http://www.w3id.org/arco/ontology/content/Character> rdf:type owl:Class ;
                                                      rdfs:subClassOf <http://www.w3id.org/arco/ontology/content/Agent> ,
                                                                      [ rdf:type owl:Restriction ;
                                                                        owl:onProperty <http://www.w3id.org/arco/ontology/content/hasCharacterRole> ;
                                                                        owl:someValuesFrom <http://www.w3id.org/arco/ontology/content/CharacterRole>
                                                                      ] ,
                                                                      [ rdf:type owl:Restriction ;
                                                                        owl:onProperty <http://www.w3id.org/arco/ontology/content/hasCharacterType> ;
                                                                        owl:someValuesFrom <http://www.w3id.org/arco/ontology/content/CharacterType>
                                                                      ] ,
                                                                      [ rdf:type owl:Restriction ;
                                                                        owl:onProperty <http://www.w3id.org/arco/ontology/content/hasFictionalType> ;
                                                                        owl:allValuesFrom [ rdf:type owl:Class ;
                                                                                            owl:unionOf ( <http://www.w3id.org/arco/ontology/content/FictionalCharacter>
                                                                                                          <http://www.w3id.org/arco/ontology/content/NonFictionalCharacter>
                                                                                                        )
                                                                                          ]
                                                                      ] ,
                                                                      [ rdf:type owl:Restriction ;
                                                                        owl:onProperty <http://www.w3id.org/arco/ontology/content/hasSocialOrigin> ;
                                                                        owl:maxQualifiedCardinality "1"^^xsd:nonNegativeInteger ;
                                                                        owl:onClass <http://www.w3id.org/arco/ontology/content/SocialOrigin>
                                                                      ] ;
                                                      rdfs:comment "This class refers to an art figure."@en .


###  http://www.w3id.org/arco/ontology/content/CharacterRole
<http://www.w3id.org/arco/ontology/content/CharacterRole> rdf:type owl:Class ;
                                                          rdfs:subClassOf <http://www.w3id.org/arco/ontology/content/Character> ;
                                                          rdfs:comment "This class refers to specific role played or filled by a character."@en .


###  http://www.w3id.org/arco/ontology/content/CharacterScope
<http://www.w3id.org/arco/ontology/content/CharacterScope> rdf:type owl:Class ;
                                                           rdfs:subClassOf <http://www.w3id.org/arco/ontology/content/Character> ;
                                                           rdfs:comment "This class refers to an identifier of a character intention."@en .


###  http://www.w3id.org/arco/ontology/content/CharacterStatus
<http://www.w3id.org/arco/ontology/content/CharacterStatus> rdf:type owl:Class ;
                                                            rdfs:subClassOf <http://www.w3id.org/arco/ontology/content/Character> ;
                                                            rdfs:comment "This class refers to social or professional character position."@en .


###  http://www.w3id.org/arco/ontology/content/CharacterType
<http://www.w3id.org/arco/ontology/content/CharacterType> rdf:type owl:Class ;
                                                          rdfs:subClassOf <http://www.w3id.org/arco/ontology/content/Character> ;
                                                          rdfs:comment "This class refers to a category of people or things having in common some characteristics."@en .


###  http://www.w3id.org/arco/ontology/content/Clergy
<http://www.w3id.org/arco/ontology/content/Clergy> rdf:type owl:Class ;
                                                   rdfs:subClassOf <http://www.w3id.org/arco/ontology/content/SocialClass> ;
                                                   owl:disjointWith <http://www.w3id.org/arco/ontology/content/Commoner> ;
                                                   rdfs:comment "This class refers to the social class people in religious orders are recognized to belong to."@en .


###  http://www.w3id.org/arco/ontology/content/Commoner
<http://www.w3id.org/arco/ontology/content/Commoner> rdf:type owl:Class ;
                                                     rdfs:subClassOf <http://www.w3id.org/arco/ontology/content/SocialClass> ;
                                                     rdfs:comment "This class refers to the social class people without any other social background are recognized to belong to."@en .


###  http://www.w3id.org/arco/ontology/content/CulturalProduct
<http://www.w3id.org/arco/ontology/content/CulturalProduct> rdf:type owl:Class ;
                                                            rdfs:comment "Goods and services that include the arts (performing arts, visual arts, architecture), heritage conservation (museums, galleries, libraries), the cultural industries (written media, broadcasting, film, recording), and festivals."@en .


###  http://www.w3id.org/arco/ontology/content/Director
<http://www.w3id.org/arco/ontology/content/Director> rdf:type owl:Class ;
                                                     rdfs:subClassOf <http://www.w3id.org/arco/ontology/content/Person> ;
                                                     rdfs:comment "This class refers to person responsible for leading teams in the artistic design and production of various kinds of visual art."@en .


###  http://www.w3id.org/arco/ontology/content/EconomicStatus
<http://www.w3id.org/arco/ontology/content/EconomicStatus> rdf:type owl:Class ;
                                                           rdfs:subClassOf <http://www.w3id.org/arco/ontology/content/SociologicalCharacteristics> ;
                                                           rdfs:comment "This class refers to the status of an agent defining its condition from an economic point of view."@en .


###  http://www.w3id.org/arco/ontology/content/Environment
<http://www.w3id.org/arco/ontology/content/Environment> rdf:type owl:Class ;
                                                        owl:equivalentClass <https://w3id.org/arco/ontology/denotative-description/Environment> ;
                                                        rdfs:subClassOf <http://www.w3id.org/arco/ontology/content/SociologicalCharacteristics> ,
                                                                        [ rdf:type owl:Restriction ;
                                                                          owl:onProperty <http://www.w3id.org/arco/ontology/content/isEnvironmentOf> ;
                                                                          owl:someValuesFrom <http://www.w3id.org/arco/ontology/content/GeographicOrigin>
                                                                        ] ;
                                                        rdfs:comment "This class refers to an environment."@en .


###  http://www.w3id.org/arco/ontology/content/EthnicGroup
<http://www.w3id.org/arco/ontology/content/EthnicGroup> rdf:type owl:Class ;
                                                        rdfs:subClassOf <http://www.w3id.org/arco/ontology/content/SociologicalCharacteristics> ,
                                                                        [ rdf:type owl:Restriction ;
                                                                          owl:onProperty <http://www.w3id.org/arco/ontology/content/defines> ;
                                                                          owl:someValuesFrom <http://www.w3id.org/arco/ontology/content/EthnicOrigin>
                                                                        ] ;
                                                        rdfs:comment "This class refers to a grouping of people who share common traits and set of traditions (ancestry, language, history, culture) that allow them to identify themselves as a distinguished group."@en .


###  http://www.w3id.org/arco/ontology/content/EthnicOrigin
<http://www.w3id.org/arco/ontology/content/EthnicOrigin> rdf:type owl:Class ;
                                                         rdfs:subClassOf <http://www.w3id.org/arco/ontology/content/Origin> ,
                                                                         [ rdf:type owl:Restriction ;
                                                                           owl:onProperty <http://www.w3id.org/arco/ontology/content/isDefinedBy> ;
                                                                           owl:someValuesFrom <http://www.w3id.org/arco/ontology/content/EthnicGroup>
                                                                         ] ;
                                                         rdfs:comment "This class refers to the peculiar trait in the origin of an individual related to its belonging to one or more ethnic groups."@en .


###  http://www.w3id.org/arco/ontology/content/FictionalCharacter
<http://www.w3id.org/arco/ontology/content/FictionalCharacter> rdf:type owl:Class ;
                                                               rdfs:subClassOf <http://www.w3id.org/arco/ontology/content/Character> ,
                                                                               [ rdf:type owl:Restriction ;
                                                                                 owl:onProperty <http://www.w3id.org/arco/ontology/content/hasPartIn> ;
                                                                                 owl:allValuesFrom <http://www.w3id.org/arco/ontology/content/FictionalPlot>
                                                                               ] ;
                                                               rdfs:comment "This class refers to fictional human or non-human character in a narrative work of art."@en .


###  http://www.w3id.org/arco/ontology/content/FictionalPlot
<http://www.w3id.org/arco/ontology/content/FictionalPlot> rdf:type owl:Class ;
                                                          rdfs:subClassOf <http://www.w3id.org/arco/ontology/content/Plot> ;
                                                          rdfs:comment "Plot based on characters or events that occurs only in stories, plays, or films and never actually existed or happened."@en .


###  http://www.w3id.org/arco/ontology/content/GeographicOrigin
<http://www.w3id.org/arco/ontology/content/GeographicOrigin> rdf:type owl:Class ;
                                                             rdfs:subClassOf <http://www.w3id.org/arco/ontology/content/Origin> ,
                                                                             [ rdf:type owl:Restriction ;
                                                                               owl:onProperty <http://www.w3id.org/arco/ontology/content/hasEnvironment> ;
                                                                               owl:allValuesFrom <http://www.w3id.org/arco/ontology/content/Environment>
                                                                             ] ;
                                                             rdfs:comment "This class refers to the peculiar trait in the origin of an individual related to its geographic provenance."@en .


###  http://www.w3id.org/arco/ontology/content/Hero
<http://www.w3id.org/arco/ontology/content/Hero> rdf:type owl:Class ;
                                                 rdfs:subClassOf <http://www.w3id.org/arco/ontology/content/CharacterType> ,
                                                                 [ rdf:type owl:Restriction ;
                                                                   owl:onProperty <http://www.w3id.org/arco/ontology/content/hasCharacterStatus> ;
                                                                   owl:someValuesFrom <http://www.w3id.org/arco/ontology/content/CharacterStatus>
                                                                 ] ,
                                                                 [ rdf:type owl:Restriction ;
                                                                   owl:onProperty <http://www.w3id.org/arco/ontology/content/hasCharacterRole> ;
                                                                   owl:allValuesFrom [ rdf:type owl:Class ;
                                                                                       owl:unionOf ( <http://www.w3id.org/arco/ontology/content/Antagonist>
                                                                                                     <http://www.w3id.org/arco/ontology/content/Protagonist>
                                                                                                   )
                                                                                     ]
                                                                 ] ,
                                                                 [ rdf:type owl:Restriction ;
                                                                   owl:onProperty <http://www.w3id.org/arco/ontology/content/hasCharacterScope> ;
                                                                   owl:allValuesFrom <http://www.w3id.org/arco/ontology/content/UniversalGood>
                                                                 ] ;
                                                 rdfs:comment "This class refers to a character who fights adversity through ingenuity, courage, or strength."@en .


###  http://www.w3id.org/arco/ontology/content/IllegalProfession
<http://www.w3id.org/arco/ontology/content/IllegalProfession> rdf:type owl:Class ;
                                                              rdfs:subClassOf <http://www.w3id.org/arco/ontology/content/Profession> ;
                                                              owl:disjointWith <http://www.w3id.org/arco/ontology/content/LegalProfession> ;
                                                              rdfs:comment "This class refers to a profession that has an illegal status."@en .


###  http://www.w3id.org/arco/ontology/content/Leading
<http://www.w3id.org/arco/ontology/content/Leading> rdf:type owl:Class ;
                                                    rdfs:subClassOf <http://www.w3id.org/arco/ontology/content/CharacterStatus> ;
                                                    rdfs:comment "This class refers to a character in a narrative that is focused on by the primary storyline."@en .


###  http://www.w3id.org/arco/ontology/content/LegalProfession
<http://www.w3id.org/arco/ontology/content/LegalProfession> rdf:type owl:Class ;
                                                            rdfs:subClassOf <http://www.w3id.org/arco/ontology/content/Profession> ;
                                                            rdfs:comment "This class refers to a profession that has a legal status."@en .


###  http://www.w3id.org/arco/ontology/content/Medium
<http://www.w3id.org/arco/ontology/content/Medium> rdf:type owl:Class ;
                                                   rdfs:subClassOf <http://www.w3id.org/arco/ontology/content/EconomicStatus> ;
                                                   rdfs:comment "This class represents an economic status of an agent that is not rich nor poor."@en .


###  http://www.w3id.org/arco/ontology/content/Movie
<http://www.w3id.org/arco/ontology/content/Movie> rdf:type owl:Class ;
                                                  rdfs:subClassOf <http://www.w3id.org/arco/ontology/content/CulturalProduct> ,
                                                                  [ rdf:type owl:Restriction ;
                                                                    owl:onProperty <https://w3id.org/arco/ontology/denotative-description/basedOn> ;
                                                                    owl:someValuesFrom <http://www.w3id.org/arco/ontology/content/Scenario>
                                                                  ] ;
                                                  rdfs:comment "A recording of moving images that tells a story and that people watch on a screen or television."@en .


###  http://www.w3id.org/arco/ontology/content/NonFictionalCharacter
<http://www.w3id.org/arco/ontology/content/NonFictionalCharacter> rdf:type owl:Class ;
                                                                  rdfs:subClassOf <http://www.w3id.org/arco/ontology/content/Character> ,
                                                                                  [ rdf:type owl:Restriction ;
                                                                                    owl:onProperty <http://www.w3id.org/arco/ontology/content/hasPartIn> ;
                                                                                    owl:allValuesFrom <http://www.w3id.org/arco/ontology/content/NonFictionalPlot>
                                                                                  ] ;
                                                                  rdfs:comment "This class refers to a non fictional human or non-human character in a narrative work of art."@en .


###  http://www.w3id.org/arco/ontology/content/NonFictionalPlot
<http://www.w3id.org/arco/ontology/content/NonFictionalPlot> rdf:type owl:Class ;
                                                             rdfs:subClassOf <http://www.w3id.org/arco/ontology/content/Plot> ;
                                                             rdfs:comment "Plot based on truth and accuracy regarding information, events, or people."@en .


###  http://www.w3id.org/arco/ontology/content/Opposing
<http://www.w3id.org/arco/ontology/content/Opposing> rdf:type owl:Class ;
                                                     rdfs:subClassOf <http://www.w3id.org/arco/ontology/content/CharacterStatus> ;
                                                     rdfs:comment "This class refers to a character in a narrative that is focused on by the primary storyline and in opposition to the leading character."@en .


###  http://www.w3id.org/arco/ontology/content/Origin
<http://www.w3id.org/arco/ontology/content/Origin> rdf:type owl:Class ;
                                                   rdfs:subClassOf <http://www.w3id.org/arco/ontology/content/SociologicalCharacteristics> ,
                                                                   [ rdf:type owl:Restriction ;
                                                                     owl:onProperty <http://www.w3id.org/arco/ontology/content/isOriginOf> ;
                                                                     owl:allValuesFrom <http://www.w3id.org/arco/ontology/content/Agent>
                                                                   ] ;
                                                   owl:disjointWith <http://www.w3id.org/arco/ontology/content/Profession> ,
                                                                    <http://www.w3id.org/arco/ontology/content/SocialClass> .


###  http://www.w3id.org/arco/ontology/content/Person
<http://www.w3id.org/arco/ontology/content/Person> rdf:type owl:Class ;
                                                   rdfs:subClassOf <http://www.w3id.org/arco/ontology/content/Agent> ;
                                                   rdfs:comment "This class refers to a human being regarded as individuals."@en .


###  http://www.w3id.org/arco/ontology/content/Plot
<http://www.w3id.org/arco/ontology/content/Plot> rdf:type owl:Class ;
                                                 rdfs:subClassOf [ rdf:type owl:Restriction ;
                                                                   owl:onProperty <https://w3id.org/arco/ontology/denotative-description/isIncludedIn> ;
                                                                   owl:someValuesFrom <http://www.w3id.org/arco/ontology/content/Scenario>
                                                                 ] ;
                                                 rdfs:comment "The main events of a play, novel, film, or similar work, devised and presented by the writer as an interrelated sequence."@en .


###  http://www.w3id.org/arco/ontology/content/Poor
<http://www.w3id.org/arco/ontology/content/Poor> rdf:type owl:Class ;
                                                 rdfs:subClassOf <http://www.w3id.org/arco/ontology/content/EconomicStatus> ;
                                                 rdfs:comment "This class represents an economic status of an agent that lacks sufficient money to live at a standard considered comfortable by society."@en .


###  http://www.w3id.org/arco/ontology/content/Profession
<http://www.w3id.org/arco/ontology/content/Profession> rdf:type owl:Class ;
                                                       owl:equivalentClass <https://w3id.org/arco/ontology/context-description/Profession> ;
                                                       rdfs:subClassOf <http://www.w3id.org/arco/ontology/content/SociologicalCharacteristics> ,
                                                                       [ rdf:type owl:Restriction ;
                                                                         owl:onProperty <http://www.w3id.org/arco/ontology/content/isProfessionOf> ;
                                                                         owl:allValuesFrom <http://www.w3id.org/arco/ontology/content/Agent>
                                                                       ] ;
                                                       owl:disjointWith <http://www.w3id.org/arco/ontology/content/SocialClass> ;
                                                       rdfs:comment "This class refers to the profession or occupation employed by an agent."@en .


###  http://www.w3id.org/arco/ontology/content/Protagonist
<http://www.w3id.org/arco/ontology/content/Protagonist> rdf:type owl:Class ;
                                                        rdfs:subClassOf <http://www.w3id.org/arco/ontology/content/CharacterRole> ,
                                                                        [ rdf:type owl:Restriction ;
                                                                          owl:onProperty <http://www.w3id.org/arco/ontology/content/hasCharacterStatus> ;
                                                                          owl:allValuesFrom <http://www.w3id.org/arco/ontology/content/Leading>
                                                                        ] ;
                                                        rdfs:comment "This class refers to the main character of a creative work."@en .


###  http://www.w3id.org/arco/ontology/content/Rich
<http://www.w3id.org/arco/ontology/content/Rich> rdf:type owl:Class ;
                                                 rdfs:subClassOf <http://www.w3id.org/arco/ontology/content/EconomicStatus> ;
                                                 rdfs:comment "This class represents an economic status of an agent that has a great deal of money or assets."@en .


###  http://www.w3id.org/arco/ontology/content/Scenario
<http://www.w3id.org/arco/ontology/content/Scenario> rdf:type owl:Class ;
                                                     rdfs:subClassOf <http://www.w3id.org/arco/ontology/content/CulturalProduct> ,
                                                                     [ rdf:type owl:Restriction ;
                                                                       owl:onProperty <https://w3id.org/arco/ontology/denotative-description/includes> ;
                                                                       owl:someValuesFrom <http://www.w3id.org/arco/ontology/content/Plot>
                                                                     ] ;
                                                     rdfs:comment "A written outline of a film, novel, or stage work giving details of the plot and individual scenes."@en .


###  http://www.w3id.org/arco/ontology/content/Screenwriter
<http://www.w3id.org/arco/ontology/content/Screenwriter> rdf:type owl:Class ;
                                                         rdfs:subClassOf <http://www.w3id.org/arco/ontology/content/Writer> ;
                                                         rdfs:comment "This class refers to a writer who wrote the script for TV, films, radio, comics or games."@en .


###  http://www.w3id.org/arco/ontology/content/Secondary
<http://www.w3id.org/arco/ontology/content/Secondary> rdf:type owl:Class ;
                                                      rdfs:subClassOf <http://www.w3id.org/arco/ontology/content/CharacterRole> ,
                                                                      [ rdf:type owl:Restriction ;
                                                                        owl:onProperty <http://www.w3id.org/arco/ontology/content/hasCharacterStatus> ;
                                                                        owl:allValuesFrom <http://www.w3id.org/arco/ontology/content/Supporting>
                                                                      ] ;
                                                      rdfs:comment "This class refers to a minor character necessary for the plot due to the key details he/she reveals."@en .


###  http://www.w3id.org/arco/ontology/content/SelfGood
<http://www.w3id.org/arco/ontology/content/SelfGood> rdf:type owl:Class ;
                                                     rdfs:subClassOf <http://www.w3id.org/arco/ontology/content/CharacterScope> ;
                                                     rdfs:comment "This class refers to the character personal advantage intention."@en .


###  http://www.w3id.org/arco/ontology/content/SocialClass
<http://www.w3id.org/arco/ontology/content/SocialClass> rdf:type owl:Class ;
                                                        rdfs:subClassOf <http://www.w3id.org/arco/ontology/content/SociologicalCharacteristics> ;
                                                        rdfs:comment "This class refers to a grouping of people identifying themselves as belonging to a specific social class within a society. The main social classes are the aristocracy, the clergy and the commoners."@en .


###  http://www.w3id.org/arco/ontology/content/SocialOrigin
<http://www.w3id.org/arco/ontology/content/SocialOrigin> rdf:type owl:Class ;
                                                         rdfs:subClassOf <http://www.w3id.org/arco/ontology/content/Origin> ,
                                                                         [ rdf:type owl:Restriction ;
                                                                           owl:onProperty <http://www.w3id.org/arco/ontology/content/isDefinedBy> ;
                                                                           owl:maxQualifiedCardinality "1"^^xsd:nonNegativeInteger ;
                                                                           owl:onClass <http://www.w3id.org/arco/ontology/content/EconomicStatus>
                                                                         ] ,
                                                                         [ rdf:type owl:Restriction ;
                                                                           owl:onProperty <http://www.w3id.org/arco/ontology/content/isDefinedBy> ;
                                                                           owl:maxQualifiedCardinality "1"^^xsd:nonNegativeInteger ;
                                                                           owl:onClass <http://www.w3id.org/arco/ontology/content/SocialClass>
                                                                         ] ;
                                                         rdfs:comment "This class refers to the peculiar trait in the origin of an individual related to its social provenance from the point of view of the social status and the social class defining them at their birth."@en .


###  http://www.w3id.org/arco/ontology/content/SociologicalCharacteristics
<http://www.w3id.org/arco/ontology/content/SociologicalCharacteristics> rdf:type owl:Class ;
                                                                        rdfs:comment "This class refers to characteristics and features able to describe an agent from a sociological point of view." .


###  http://www.w3id.org/arco/ontology/content/SupernaturalBeing
<http://www.w3id.org/arco/ontology/content/SupernaturalBeing> rdf:type owl:Class ;
                                                              rdfs:subClassOf <http://www.w3id.org/arco/ontology/content/Agent> ;
                                                              rdfs:comment "This class refers to kind of being from religion, mythology or folklore."@en .


###  http://www.w3id.org/arco/ontology/content/Supporting
<http://www.w3id.org/arco/ontology/content/Supporting> rdf:type owl:Class ;
                                                       rdfs:subClassOf <http://www.w3id.org/arco/ontology/content/CharacterStatus> ;
                                                       rdfs:comment "This class refers to a character in a narrative that is not focused on by the primary storyline."@en .


###  http://www.w3id.org/arco/ontology/content/TvSeries
<http://www.w3id.org/arco/ontology/content/TvSeries> rdf:type owl:Class ;
                                                     rdfs:subClassOf <http://www.w3id.org/arco/ontology/content/CulturalProduct> ,
                                                                     [ rdf:type owl:Restriction ;
                                                                       owl:onProperty <https://w3id.org/arco/ontology/denotative-description/basedOn> ;
                                                                       owl:someValuesFrom <http://www.w3id.org/arco/ontology/content/Scenario>
                                                                     ] ;
                                                     rdfs:comment "A group of programs created or adapted for television broadcast with a common series title."@en .


###  http://www.w3id.org/arco/ontology/content/UniversalBad
<http://www.w3id.org/arco/ontology/content/UniversalBad> rdf:type owl:Class ;
                                                         rdfs:subClassOf <http://www.w3id.org/arco/ontology/content/CharacterScope> ;
                                                         rdfs:comment "An action that is against the interest of the world, applicable to all cases (humans, animals, enviroment etc.)."@en .


###  http://www.w3id.org/arco/ontology/content/UniversalGood
<http://www.w3id.org/arco/ontology/content/UniversalGood> rdf:type owl:Class ;
                                                          rdfs:subClassOf <http://www.w3id.org/arco/ontology/content/CharacterScope> ;
                                                          rdfs:comment "An action that is in the interest of the world, applicable to all cases (humans, animals, enviroment etc.)."@en .


###  http://www.w3id.org/arco/ontology/content/Villain
<http://www.w3id.org/arco/ontology/content/Villain> rdf:type owl:Class ;
                                                    rdfs:subClassOf <http://www.w3id.org/arco/ontology/content/CharacterType> ,
                                                                    [ rdf:type owl:Restriction ;
                                                                      owl:onProperty <http://www.w3id.org/arco/ontology/content/hasCharacterStatus> ;
                                                                      owl:someValuesFrom <http://www.w3id.org/arco/ontology/content/CharacterStatus>
                                                                    ] ,
                                                                    [ rdf:type owl:Restriction ;
                                                                      owl:onProperty <http://www.w3id.org/arco/ontology/content/hasCharacterRole> ;
                                                                      owl:allValuesFrom [ rdf:type owl:Class ;
                                                                                          owl:unionOf ( <http://www.w3id.org/arco/ontology/content/Antagonist>
                                                                                                        <http://www.w3id.org/arco/ontology/content/Protagonist>
                                                                                                      )
                                                                                        ]
                                                                    ] ,
                                                                    [ rdf:type owl:Restriction ;
                                                                      owl:onProperty <http://www.w3id.org/arco/ontology/content/hasCharacterScope> ;
                                                                      owl:allValuesFrom <http://www.w3id.org/arco/ontology/content/UniversalBad>
                                                                    ] ;
                                                    rdfs:comment "This class refers to a character whose evil actions or motives are important to the plot."@en .


###  http://www.w3id.org/arco/ontology/content/Writer
<http://www.w3id.org/arco/ontology/content/Writer> rdf:type owl:Class ;
                                                   rdfs:subClassOf <http://www.w3id.org/arco/ontology/content/Person> ;
                                                   rdfs:comment "This class refers to person who uses written words to communicate ideas and to produce works of literature."@en .


#################################################################
#    General axioms
#################################################################

[ rdf:type owl:AllDisjointClasses ;
  owl:members ( <http://www.w3id.org/arco/ontology/content/Animal>
                <http://www.w3id.org/arco/ontology/content/Character>
                <http://www.w3id.org/arco/ontology/content/Person>
                <http://www.w3id.org/arco/ontology/content/SupernaturalBeing>
              )
] .


[ rdf:type owl:AllDisjointClasses ;
  owl:members ( <http://www.w3id.org/arco/ontology/content/EthnicOrigin>
                <http://www.w3id.org/arco/ontology/content/GeographicOrigin>
                <http://www.w3id.org/arco/ontology/content/SocialOrigin>
              )
] .


[ rdf:type owl:AllDisjointClasses ;
  owl:members ( <http://www.w3id.org/arco/ontology/content/Medium>
                <http://www.w3id.org/arco/ontology/content/Poor>
                <http://www.w3id.org/arco/ontology/content/Rich>
              )
] .


[ rdf:type owl:AllDisjointClasses ;
  owl:members ( <http://www.w3id.org/arco/ontology/content/Movie>
                <http://www.w3id.org/arco/ontology/content/Scenario>
                <http://www.w3id.org/arco/ontology/content/TvSeries>
              )
] .


###  Generated by the OWL API (version 5.1.14) https://github.com/owlcs/owlapi/
