@prefix : <http://www.semanticweb.org/ontologies/2021/1/content#> .
@prefix owl: <http://www.w3.org/2002/07/owl#> .
@prefix rdf: <http://www.w3.org/1999/02/22-rdf-syntax-ns#> .
@prefix xml: <http://www.w3.org/XML/1998/namespace> .
@prefix xsd: <http://www.w3.org/2001/XMLSchema#> .
@prefix cont: <http://www.semanticweb.org/ontologies/2021/1/content#> .
@prefix rdfs: <http://www.w3.org/2000/01/rdf-schema#> .
@base <http://www.semanticweb.org/ontologies/2021/1/content> .

<http://www.semanticweb.org/ontologies/2021/1/content> rdf:type owl:Ontology ;
                                                        owl:imports <https://w3id.org/arco/ontology/context-description> ,
                                                                    <https://w3id.org/arco/ontology/denotative-description> .

#################################################################
#    Object Properties
#################################################################

###  http://www.semanticweb.org/ontologies/2021/1/content#defines
cont:defines rdf:type owl:ObjectProperty ;
             rdfs:comment "This property define the act of attaching a meaning to a term."@en .


###  http://www.semanticweb.org/ontologies/2021/1/content#hasAuthor
cont:hasAuthor rdf:type owl:ObjectProperty ;
               owl:inverseOf cont:isAuthorOf ;
               rdfs:comment "This property links any written work to its creator or originator."@en .


###  http://www.semanticweb.org/ontologies/2021/1/content#hasBusinessPartner
cont:hasBusinessPartner rdf:type owl:ObjectProperty ;
                        rdfs:subPropertyOf cont:isRelatedTo ;
                        rdf:type owl:SymmetricProperty ;
                        rdfs:comment "This property defines a business relations bwtween two agents."@en .


###  http://www.semanticweb.org/ontologies/2021/1/content#hasCharacter
cont:hasCharacter rdf:type owl:ObjectProperty ;
                  owl:inverseOf cont:isCharacterOf .


###  http://www.semanticweb.org/ontologies/2021/1/content#hasCharacterRole
cont:hasCharacterRole rdf:type owl:ObjectProperty ;
                      rdfs:subPropertyOf cont:hasType ;
                      owl:inverseOf cont:isCharacterRole ;
                      rdfs:comment "This property defines character’s role as protagonist, antagonist or secondary."@en .


###  http://www.semanticweb.org/ontologies/2021/1/content#hasCharacterScope
cont:hasCharacterScope rdf:type owl:ObjectProperty ;
                       rdfs:subPropertyOf cont:hasType ;
                       owl:inverseOf cont:isCharacterScope ;
                       rdfs:comment "This property defines character’s scope as universal good, universal bad or self good."@en .


###  http://www.semanticweb.org/ontologies/2021/1/content#hasCharacterStatus
cont:hasCharacterStatus rdf:type owl:ObjectProperty ;
                        rdfs:subPropertyOf cont:hasType ;
                        owl:inverseOf cont:isCharacterStatus ;
                        rdfs:comment "This property defines character’s status as leading, opposing or supporting."@en .


###  http://www.semanticweb.org/ontologies/2021/1/content#hasCharacterType
cont:hasCharacterType rdf:type owl:ObjectProperty ;
                      rdfs:subPropertyOf cont:hasType ;
                      owl:inverseOf cont:isCharacterType ;
                      rdfs:comment "This property defines character’s type as hero, antihero, or villain."@en .


###  http://www.semanticweb.org/ontologies/2021/1/content#hasChild
cont:hasChild rdf:type owl:ObjectProperty ;
              rdfs:subPropertyOf cont:hasRelative ;
              owl:inverseOf cont:hasParent ;
              rdfs:comment "This property links an agent that is parent to another agent."@en .


###  http://www.semanticweb.org/ontologies/2021/1/content#hasEmployee
cont:hasEmployee rdf:type owl:ObjectProperty ;
                 rdfs:subPropertyOf cont:isRelatedTo ;
                 owl:inverseOf cont:hasEmployer ;
                 rdfs:comment "This property links an employer to its employee."@en .


###  http://www.semanticweb.org/ontologies/2021/1/content#hasEmployer
cont:hasEmployer rdf:type owl:ObjectProperty ;
                 rdfs:subPropertyOf cont:isRelatedTo ;
                 rdfs:comment "This property links an employee to its employer."@en .


###  http://www.semanticweb.org/ontologies/2021/1/content#hasEnvironment
cont:hasEnvironment rdf:type owl:ObjectProperty ;
                    rdfs:subPropertyOf cont:hasSociologicalCharacteristic ;
                    rdfs:comment "This property links an agent to an environment."@en .


###  http://www.semanticweb.org/ontologies/2021/1/content#hasEthnicGroup
cont:hasEthnicGroup rdf:type owl:ObjectProperty ;
                    rdfs:subPropertyOf cont:hasSociologicalCharacteristic ;
                    owl:inverseOf cont:isEthnicGroupOf ;
                    rdfs:comment "This property links an agent to an ethnic group."@en .


###  http://www.semanticweb.org/ontologies/2021/1/content#hasEthnicOrigin
cont:hasEthnicOrigin rdf:type owl:ObjectProperty ;
                     rdfs:subPropertyOf cont:hasOrigin ;
                     owl:inverseOf cont:isEthnicOriginOf ;
                     rdfs:comment "This property defines the origin an agent has from an ethnic point of view."@en .


###  http://www.semanticweb.org/ontologies/2021/1/content#hasFictionalType
cont:hasFictionalType rdf:type owl:ObjectProperty ;
                      rdfs:subPropertyOf cont:hasType ;
                      owl:inverseOf cont:isFictionalType ;
                      rdfs:comment "This property defines fictional character’s type as fictional or non fictional."@en .


###  http://www.semanticweb.org/ontologies/2021/1/content#hasGeographicOrigin
cont:hasGeographicOrigin rdf:type owl:ObjectProperty ;
                         rdfs:subPropertyOf cont:hasOrigin ;
                         owl:inverseOf cont:isGeographicOriginOf ;
                         rdfs:comment "This property defines the origin an agent has from a geographic point of view."@en .


###  http://www.semanticweb.org/ontologies/2021/1/content#hasOrigin
cont:hasOrigin rdf:type owl:ObjectProperty ;
               rdfs:subPropertyOf cont:hasSociologicalCharacteristic ;
               rdfs:comment "This property defines the origin an agent has."@en .


###  http://www.semanticweb.org/ontologies/2021/1/content#hasParent
cont:hasParent rdf:type owl:ObjectProperty ;
               rdfs:subPropertyOf cont:hasRelative ;
               rdfs:comment "This property link an agent that is child to another agent."@en .


###  http://www.semanticweb.org/ontologies/2021/1/content#hasPartIn
cont:hasPartIn rdf:type owl:ObjectProperty ;
               rdfs:comment "To be involved in, to be a factor in."@en .


###  http://www.semanticweb.org/ontologies/2021/1/content#hasProfession
cont:hasProfession rdf:type owl:ObjectProperty ;
                   rdfs:subPropertyOf cont:hasSociologicalCharacteristic ;
                   rdfs:comment "This property links an agent to a profession."@en .


###  http://www.semanticweb.org/ontologies/2021/1/content#hasRelative
cont:hasRelative rdf:type owl:ObjectProperty ;
                 rdfs:subPropertyOf cont:isRelatedTo ;
                 rdf:type owl:SymmetricProperty ;
                 rdfs:comment "This property links two agents connected by blood or marriage."@en .


###  http://www.semanticweb.org/ontologies/2021/1/content#hasRole
cont:hasRole rdf:type owl:ObjectProperty ;
             owl:inverseOf cont:isRole ;
             rdfs:comment "This property defines the role of character in a play."@en .


###  http://www.semanticweb.org/ontologies/2021/1/content#hasSocialOrigin
cont:hasSocialOrigin rdf:type owl:ObjectProperty ;
                     rdfs:subPropertyOf cont:hasOrigin ;
                     rdf:type owl:FunctionalProperty ;
                     rdfs:comment "This property defines the origin an agent has from a social point of view."@en .


###  http://www.semanticweb.org/ontologies/2021/1/content#hasSociologicalCharacteristic
cont:hasSociologicalCharacteristic rdf:type owl:ObjectProperty ;
                                   owl:inverseOf cont:isSociologicalCharacteristicOf ;
                                   rdfs:comment "This property defines a sociological characteristic that can be described as belonging to an agent."@en .


###  http://www.semanticweb.org/ontologies/2021/1/content#hasSpinOff
cont:hasSpinOff rdf:type owl:ObjectProperty ;
                owl:inverseOf cont:isSpinOffOf ;
                rdfs:comment "This property links a TV serie to another TV serie in which a secondary character in the first show becomes the protagonist."@en .


###  http://www.semanticweb.org/ontologies/2021/1/content#hasType
cont:hasType rdf:type owl:ObjectProperty ;
             owl:inverseOf cont:isType ;
             rdfs:comment "This property defines the typology of character depicted as human, animal or supernatural one."@en .


###  http://www.semanticweb.org/ontologies/2021/1/content#isAuthorOf
cont:isAuthorOf rdf:type owl:ObjectProperty ;
                rdfs:comment "This property links a creator or originator to its written work."@en .


###  http://www.semanticweb.org/ontologies/2021/1/content#isBasedOn
cont:isBasedOn rdf:type owl:ObjectProperty ,
                        owl:FunctionalProperty ,
                        owl:InverseFunctionalProperty ;
               rdfs:comment "This property defines a character that is based on or inspired to a real or invented person, animal or supernatural being."@en .


###  http://www.semanticweb.org/ontologies/2021/1/content#isCharacterOf
cont:isCharacterOf rdf:type owl:ObjectProperty .


###  http://www.semanticweb.org/ontologies/2021/1/content#isCharacterRole
cont:isCharacterRole rdf:type owl:ObjectProperty ;
                     rdfs:subPropertyOf cont:isType ;
                     rdfs:comment "This property defines protagonist, antagonist and secondary as character’s role."@en .


###  http://www.semanticweb.org/ontologies/2021/1/content#isCharacterScope
cont:isCharacterScope rdf:type owl:ObjectProperty ;
                      rdfs:subPropertyOf cont:isType ;
                      rdfs:comment "This property defines universal good, universal bad and self good as character’s scope."@en .


###  http://www.semanticweb.org/ontologies/2021/1/content#isCharacterStatus
cont:isCharacterStatus rdf:type owl:ObjectProperty ;
                       rdfs:subPropertyOf cont:isType ;
                       rdfs:comment "This property defines leading, opposing, and supporting as character’s status."@en .


###  http://www.semanticweb.org/ontologies/2021/1/content#isCharacterType
cont:isCharacterType rdf:type owl:ObjectProperty ;
                     rdfs:subPropertyOf cont:isType ;
                     rdfs:comment "This property defines hero, antihero, and villain as character’s type."@en .


###  http://www.semanticweb.org/ontologies/2021/1/content#isDefinedBy
cont:isDefinedBy rdf:type owl:ObjectProperty ;
                 rdfs:comment "This property defines the meaning that is attached to a term."@en .


###  http://www.semanticweb.org/ontologies/2021/1/content#isEnvironmentOf
cont:isEnvironmentOf rdf:type owl:ObjectProperty ;
                     rdfs:subPropertyOf cont:isSociologicalCharacteristicOf ;
                     rdfs:comment "This property links an environment to an agent."@en .


###  http://www.semanticweb.org/ontologies/2021/1/content#isEthnicGroupOf
cont:isEthnicGroupOf rdf:type owl:ObjectProperty ;
                     rdfs:subPropertyOf cont:isSociologicalCharacteristicOf ;
                     rdfs:comment "This property links an ethnic group to an agent."@en .


###  http://www.semanticweb.org/ontologies/2021/1/content#isEthnicOriginOf
cont:isEthnicOriginOf rdf:type owl:ObjectProperty ;
                      rdfs:subPropertyOf cont:isOriginOf ;
                      rdfs:comment "This property defines the origin referring to an agent from an ethnic point of view."@en .


###  http://www.semanticweb.org/ontologies/2021/1/content#isFictionalType
cont:isFictionalType rdf:type owl:ObjectProperty ;
                     rdfs:subPropertyOf cont:isType ;
                     rdfs:comment "This property defines fictional and non fictional as character’s fictional type."@en .


###  http://www.semanticweb.org/ontologies/2021/1/content#isGeographicOriginOf
cont:isGeographicOriginOf rdf:type owl:ObjectProperty ;
                          rdfs:subPropertyOf cont:isOriginOf ;
                          rdfs:comment "This property defines the origin referring to an agent from a geographic point of view."@en .


###  http://www.semanticweb.org/ontologies/2021/1/content#isKilledBy
cont:isKilledBy rdf:type owl:ObjectProperty ;
                owl:inverseOf cont:kills ;
                rdfs:comment "This property links two agents in which the first one is killed by the second one."@en .


###  http://www.semanticweb.org/ontologies/2021/1/content#isOriginOf
cont:isOriginOf rdf:type owl:ObjectProperty ;
                rdfs:subPropertyOf cont:isSociologicalCharacteristicOf ;
                rdfs:comment "This property defines the origin referring to an agent."@en .


###  http://www.semanticweb.org/ontologies/2021/1/content#isPlayedBy
cont:isPlayedBy rdf:type owl:ObjectProperty ;
                owl:inverseOf cont:plays ;
                rdfs:comment "This property defines a character that is interpreted by an actor."@en .


###  http://www.semanticweb.org/ontologies/2021/1/content#isProfessionOf
cont:isProfessionOf rdf:type owl:ObjectProperty ;
                    rdfs:subPropertyOf cont:isSociologicalCharacteristicOf ;
                    rdfs:comment "This property link a profession to an agent."@en .


###  http://www.semanticweb.org/ontologies/2021/1/content#isRelatedTo
cont:isRelatedTo rdf:type owl:ObjectProperty ,
                          owl:SymmetricProperty ;
                 rdfs:comment "This property defines a personal relations between two agents."@en .


###  http://www.semanticweb.org/ontologies/2021/1/content#isRole
cont:isRole rdf:type owl:ObjectProperty ;
            rdfs:comment "This property defines a character by its role in a play."@en .


###  http://www.semanticweb.org/ontologies/2021/1/content#isSocialOriginOf
cont:isSocialOriginOf rdf:type owl:ObjectProperty ;
                      rdfs:subPropertyOf cont:isOriginOf ;
                      rdfs:comment "This property defines the origin referring to an agent from a social point of view."@en .


###  http://www.semanticweb.org/ontologies/2021/1/content#isSociologicalCharacteristicOf
cont:isSociologicalCharacteristicOf rdf:type owl:ObjectProperty ;
                                    rdfs:comment "This property defines a sociological characteristic that refers to an agent." .


###  http://www.semanticweb.org/ontologies/2021/1/content#isSpinOffOf
cont:isSpinOffOf rdf:type owl:ObjectProperty ;
                 rdfs:comment "This property links a TV serie to another TV serie in which the protagonist played a secondary role."@en .


###  http://www.semanticweb.org/ontologies/2021/1/content#isType
cont:isType rdf:type owl:ObjectProperty ;
            rdfs:comment "This property defines human, animal or supernatural being as typology of character."@en .


###  http://www.semanticweb.org/ontologies/2021/1/content#kills
cont:kills rdf:type owl:ObjectProperty ;
           rdfs:comment "This property links two agents in which the first one kills the second one."@en .


###  http://www.semanticweb.org/ontologies/2021/1/content#plays
cont:plays rdf:type owl:ObjectProperty ;
           rdfs:comment "This property defines an actor that interprets a character."@en .


#################################################################
#    Data properties
#################################################################

###  http://www.semanticweb.org/ontologies/2021/1/content#hasAlternativeName
cont:hasAlternativeName rdf:type owl:DatatypeProperty ;
                        rdfs:subPropertyOf cont:hasName ;
                        rdfs:range xsd:string .


###  http://www.semanticweb.org/ontologies/2021/1/content#hasBirthDate
cont:hasBirthDate rdf:type owl:DatatypeProperty ;
                  rdfs:range xsd:dateTime ;
                  rdfs:comment "This property associates an agent to the day of its birth."@en .


###  http://www.semanticweb.org/ontologies/2021/1/content#hasDeathDate
cont:hasDeathDate rdf:type owl:DatatypeProperty ;
                  rdfs:range xsd:dateTime ;
                  rdfs:comment "This property associates an agent to the day of its death."@en .


###  http://www.semanticweb.org/ontologies/2021/1/content#hasFirstName
cont:hasFirstName rdf:type owl:DatatypeProperty ;
                  rdfs:subPropertyOf cont:hasName ;
                  rdfs:comment "This property links an agent to its first name."@en .


###  http://www.semanticweb.org/ontologies/2021/1/content#hasLastName
cont:hasLastName rdf:type owl:DatatypeProperty ;
                 rdfs:subPropertyOf cont:hasName ;
                 rdfs:comment "This property links an agent to its last name."@en .


###  http://www.semanticweb.org/ontologies/2021/1/content#hasName
cont:hasName rdf:type owl:DatatypeProperty ;
             rdfs:range xsd:string ;
             rdfs:comment "This property links an agent to its name."@en .


###  http://www.semanticweb.org/ontologies/2021/1/content#hasNickname
cont:hasNickname rdf:type owl:DatatypeProperty ;
                 rdfs:subPropertyOf cont:hasAlternativeName ;
                 rdfs:range xsd:string ;
                 rdfs:comment "This property links an agent to its nickname."@en .


###  http://www.semanticweb.org/ontologies/2021/1/content#hasPlaceOfBirth
cont:hasPlaceOfBirth rdf:type owl:DatatypeProperty ;
                     rdfs:comment "This property links an agent to the geografical place in which it was born."@en .


###  http://www.semanticweb.org/ontologies/2021/1/content#hasPlaceOfDeath
cont:hasPlaceOfDeath rdf:type owl:DatatypeProperty ;
                     rdfs:comment "This property links an agent to the geografical place in which it died."@en .


###  http://www.semanticweb.org/ontologies/2021/1/content#hasPlaceOfLiving
cont:hasPlaceOfLiving rdf:type owl:DatatypeProperty ;
                      rdfs:comment "This property links an agent to the geografical place in which it lives."@en .


###  http://www.semanticweb.org/ontologies/2021/1/content#hasPseudonym
cont:hasPseudonym rdf:type owl:DatatypeProperty ;
                  rdfs:subPropertyOf cont:hasAlternativeName ;
                  rdfs:range xsd:string ;
                  rdfs:comment "This property links an agent to its pseudonym."@en .


###  http://www.semanticweb.org/ontologies/2021/1/content#hasSex
cont:hasSex rdf:type owl:DatatypeProperty ;
            rdfs:range xsd:string ;
            rdfs:comment "This property links an agent to its biological sex."@en .


#################################################################
#    Classes
#################################################################

###  http://dati.beniculturali.it/cis/CulturalEntity
<http://dati.beniculturali.it/cis/CulturalEntity> owl:equivalentClass cont:CulturalProduct .


###  http://dati.gov.it/onto/dcatapit#Agent
<http://dati.gov.it/onto/dcatapit#Agent> owl:equivalentClass cont:Agent .


###  http://www.semanticweb.org/ontologies/2021/1/content#Actor
cont:Actor rdf:type owl:Class ;
           rdfs:subClassOf cont:Person ;
           rdfs:comment "This class refers to a person who’s profession is acting on stage, films, or television."@en .


###  http://www.semanticweb.org/ontologies/2021/1/content#Agent
cont:Agent rdf:type owl:Class ;
           owl:equivalentClass <https://w3id.org/italia/onto/l0/Agent> ;
           rdfs:subClassOf owl:Thing ,
                           [ rdf:type owl:Restriction ;
                             owl:onProperty cont:hasProfession ;
                             owl:someValuesFrom cont:Profession
                           ] ,
                           [ rdf:type owl:Restriction ;
                             owl:onProperty cont:hasSocialOrigin ;
                             owl:maxQualifiedCardinality "1"^^xsd:nonNegativeInteger ;
                             owl:onClass cont:SocialOrigin
                           ] ;
           owl:disjointWith cont:SociologicalCharacteristics .


###  http://www.semanticweb.org/ontologies/2021/1/content#Animal
cont:Animal rdf:type owl:Class ;
            rdfs:subClassOf cont:Agent ;
            rdfs:comment "This class refers to living organism that feeds on organic matter."@en .


###  http://www.semanticweb.org/ontologies/2021/1/content#Antagonist
cont:Antagonist rdf:type owl:Class ;
                rdfs:subClassOf cont:CharacterRole ,
                                [ rdf:type owl:Restriction ;
                                  owl:onProperty cont:hasCharacterStatus ;
                                  owl:allValuesFrom cont:Opposing
                                ] ;
                rdfs:comment "This class refers to a character of a work actively opposing the protagonist."@en .


###  http://www.semanticweb.org/ontologies/2021/1/content#AntiHero
cont:AntiHero rdf:type owl:Class ;
              rdfs:subClassOf cont:CharacterType ,
                              [ rdf:type owl:Restriction ;
                                owl:onProperty cont:hasCharacterStatus ;
                                owl:someValuesFrom cont:CharacterStatus
                              ] ,
                              [ rdf:type owl:Restriction ;
                                owl:onProperty cont:hasCharacterRole ;
                                owl:allValuesFrom [ rdf:type owl:Class ;
                                                    owl:unionOf ( cont:Antagonist
                                                                  cont:CharacterStatus
                                                                  cont:Protagonist
                                                                  cont:Secondary
                                                                )
                                                  ]
                              ] ,
                              [ rdf:type owl:Restriction ;
                                owl:onProperty cont:hasCharacterScope ;
                                owl:allValuesFrom cont:SelfGood
                              ] ;
              rdfs:comment "This class refers to a leading character in a film, book or play, who is devoid of heroic qualities."@en .


###  http://www.semanticweb.org/ontologies/2021/1/content#Aristocracy
cont:Aristocracy rdf:type owl:Class ;
                 rdfs:subClassOf cont:SocialClass ;
                 owl:disjointWith cont:Clergy ,
                                  cont:Commoner ;
                 rdfs:comment "This class refers to the social class aristocrats are recognized to belong to."@en .


###  http://www.semanticweb.org/ontologies/2021/1/content#Author
cont:Author rdf:type owl:Class ;
            rdfs:subClassOf cont:Writer ;
            rdfs:comment "This class refers to a writer of any written work."@en .


###  http://www.semanticweb.org/ontologies/2021/1/content#Character
cont:Character rdf:type owl:Class ;
               rdfs:subClassOf cont:Agent ,
                               [ rdf:type owl:Restriction ;
                                 owl:onProperty cont:hasCharacterRole ;
                                 owl:someValuesFrom cont:CharacterRole
                               ] ,
                               [ rdf:type owl:Restriction ;
                                 owl:onProperty cont:hasCharacterType ;
                                 owl:someValuesFrom cont:CharacterType
                               ] ,
                               [ rdf:type owl:Restriction ;
                                 owl:onProperty cont:hasFictionalType ;
                                 owl:allValuesFrom [ rdf:type owl:Class ;
                                                     owl:unionOf ( cont:FictionalCharacter
                                                                   cont:NonFictionalCharacter
                                                                 )
                                                   ]
                               ] ,
                               [ rdf:type owl:Restriction ;
                                 owl:onProperty cont:hasSocialOrigin ;
                                 owl:maxQualifiedCardinality "1"^^xsd:nonNegativeInteger ;
                                 owl:onClass cont:SocialOrigin
                               ] ;
               rdfs:comment "This class refers to an art figure."@en .


###  http://www.semanticweb.org/ontologies/2021/1/content#CharacterRole
cont:CharacterRole rdf:type owl:Class ;
                   rdfs:subClassOf cont:Character ;
                   rdfs:comment "This class refers to specific role played or filled by a character."@en .


###  http://www.semanticweb.org/ontologies/2021/1/content#CharacterScope
cont:CharacterScope rdf:type owl:Class ;
                    rdfs:subClassOf cont:Character ;
                    rdfs:comment "This class refers to an identifier of a character intention."@en .


###  http://www.semanticweb.org/ontologies/2021/1/content#CharacterStatus
cont:CharacterStatus rdf:type owl:Class ;
                     rdfs:subClassOf cont:Character ;
                     rdfs:comment "This class refers to social or professional character position."@en .


###  http://www.semanticweb.org/ontologies/2021/1/content#CharacterType
cont:CharacterType rdf:type owl:Class ;
                   rdfs:subClassOf cont:Character ;
                   rdfs:comment "This class refers to a category of people or things having in common some characteristics."@en .


###  http://www.semanticweb.org/ontologies/2021/1/content#Clergy
cont:Clergy rdf:type owl:Class ;
            rdfs:subClassOf cont:SocialClass ;
            owl:disjointWith cont:Commoner ;
            rdfs:comment "This class refers to the social class people in religious orders are recognized to belong to."@en .


###  http://www.semanticweb.org/ontologies/2021/1/content#Commoner
cont:Commoner rdf:type owl:Class ;
              rdfs:subClassOf cont:SocialClass ;
              rdfs:comment "This class refers to the social class people without any other social background are recognized to belong to."@en .


###  http://www.semanticweb.org/ontologies/2021/1/content#CulturalProduct
cont:CulturalProduct rdf:type owl:Class ;
                     rdfs:comment "Goods and services that include the arts (performing arts, visual arts, architecture), heritage conservation (museums, galleries, libraries), the cultural industries (written media, broadcasting, film, recording), and festivals."@en .


###  http://www.semanticweb.org/ontologies/2021/1/content#Director
cont:Director rdf:type owl:Class ;
              rdfs:subClassOf cont:Person ;
              rdfs:comment "This class refers to person responsible for leading teams in the artistic design and production of various kinds of visual art."@en .


###  http://www.semanticweb.org/ontologies/2021/1/content#EconomicStatus
cont:EconomicStatus rdf:type owl:Class ;
                    rdfs:subClassOf cont:SociologicalCharacteristics ;
                    rdfs:comment "This class refers to the status of an agent defining its condition from an economic point of view."@en .


###  http://www.semanticweb.org/ontologies/2021/1/content#Environment
cont:Environment rdf:type owl:Class ;
                 owl:equivalentClass <https://w3id.org/arco/ontology/denotative-description/Environment> ;
                 rdfs:subClassOf cont:SociologicalCharacteristics ,
                                 [ rdf:type owl:Restriction ;
                                   owl:onProperty cont:isEnvironmentOf ;
                                   owl:someValuesFrom cont:GeographicOrigin
                                 ] ;
                 rdfs:comment "This class refers to an environment."@en .


###  http://www.semanticweb.org/ontologies/2021/1/content#EthnicGroup
cont:EthnicGroup rdf:type owl:Class ;
                 rdfs:subClassOf cont:SociologicalCharacteristics ,
                                 [ rdf:type owl:Restriction ;
                                   owl:onProperty cont:defines ;
                                   owl:someValuesFrom cont:EthnicOrigin
                                 ] ;
                 rdfs:comment "This class refers to a grouping of people who share common traits and set of traditions (ancestry, language, history, culture) that allow them to identify themselves as a distinguished group."@en .


###  http://www.semanticweb.org/ontologies/2021/1/content#EthnicOrigin
cont:EthnicOrigin rdf:type owl:Class ;
                  rdfs:subClassOf cont:Origin ,
                                  [ rdf:type owl:Restriction ;
                                    owl:onProperty cont:isDefinedBy ;
                                    owl:someValuesFrom cont:EthnicGroup
                                  ] ;
                  rdfs:comment "This class refers to the peculiar trait in the origin of an individual related to its belonging to one or more ethnic groups."@en .


###  http://www.semanticweb.org/ontologies/2021/1/content#FictionalCharacter
cont:FictionalCharacter rdf:type owl:Class ;
                        rdfs:subClassOf cont:Character ,
                                        [ rdf:type owl:Restriction ;
                                          owl:onProperty cont:hasPartIn ;
                                          owl:allValuesFrom cont:FictionalPlot
                                        ] ;
                        rdfs:comment "This class refers to fictional human or non-human character in a narrative work of art."@en .


###  http://www.semanticweb.org/ontologies/2021/1/content#FictionalPlot
cont:FictionalPlot rdf:type owl:Class ;
                   rdfs:subClassOf cont:Plot ;
                   rdfs:comment "Plot based on characters or events that occurs only in stories, plays, or films and never actually existed or happened."@en .


###  http://www.semanticweb.org/ontologies/2021/1/content#GeographicOrigin
cont:GeographicOrigin rdf:type owl:Class ;
                      rdfs:subClassOf cont:Origin ,
                                      [ rdf:type owl:Restriction ;
                                        owl:onProperty cont:hasEnvironment ;
                                        owl:allValuesFrom cont:Environment
                                      ] ;
                      rdfs:comment "This class refers to the peculiar trait in the origin of an individual related to its geographic provenance."@en .


###  http://www.semanticweb.org/ontologies/2021/1/content#Hero
cont:Hero rdf:type owl:Class ;
          rdfs:subClassOf cont:CharacterType ,
                          [ rdf:type owl:Restriction ;
                            owl:onProperty cont:hasCharacterStatus ;
                            owl:someValuesFrom cont:CharacterStatus
                          ] ,
                          [ rdf:type owl:Restriction ;
                            owl:onProperty cont:hasCharacterRole ;
                            owl:allValuesFrom [ rdf:type owl:Class ;
                                                owl:unionOf ( cont:Antagonist
                                                              cont:Protagonist
                                                            )
                                              ]
                          ] ,
                          [ rdf:type owl:Restriction ;
                            owl:onProperty cont:hasCharacterScope ;
                            owl:allValuesFrom cont:UniversalGood
                          ] ;
          rdfs:comment "This class refers to a character who fights adversity through ingenuity, courage, or strength."@en .


###  http://www.semanticweb.org/ontologies/2021/1/content#IllegalProfession
cont:IllegalProfession rdf:type owl:Class ;
                       rdfs:subClassOf cont:Profession ;
                       owl:disjointWith cont:LegalProfession ;
                       rdfs:comment "This class refers to a profession that has an illegal status."@en .


###  http://www.semanticweb.org/ontologies/2021/1/content#Leading
cont:Leading rdf:type owl:Class ;
             rdfs:subClassOf cont:CharacterStatus ;
             rdfs:comment "This class refers to a character in a narrative that is focused on by the primary storyline."@en .


###  http://www.semanticweb.org/ontologies/2021/1/content#LegalProfession
cont:LegalProfession rdf:type owl:Class ;
                     rdfs:subClassOf cont:Profession ;
                     rdfs:comment "This class refers to a profession that has a legal status."@en .


###  http://www.semanticweb.org/ontologies/2021/1/content#LiteraryWork
cont:LiteraryWork rdf:type owl:Class ;
                  rdfs:subClassOf cont:CulturalProduct ;
                  rdfs:comment "Imaginative or creative writing textual work, with or without illustrations, published or nonpublished."@en .


###  http://www.semanticweb.org/ontologies/2021/1/content#Medium
cont:Medium rdf:type owl:Class ;
            rdfs:subClassOf cont:EconomicStatus ;
            rdfs:comment "This class represents an economic status of an agent that is not rich nor poor."@en .


###  http://www.semanticweb.org/ontologies/2021/1/content#Movie
cont:Movie rdf:type owl:Class ;
           rdfs:subClassOf cont:Scenario ;
           rdfs:comment "A recording of moving images that tells a story and that people watch on a screen or television."@en .


###  http://www.semanticweb.org/ontologies/2021/1/content#NonFictionalCharacter
cont:NonFictionalCharacter rdf:type owl:Class ;
                           rdfs:subClassOf cont:Character ,
                                           [ rdf:type owl:Restriction ;
                                             owl:onProperty cont:hasPartIn ;
                                             owl:allValuesFrom cont:NonFictionalPlot
                                           ] ;
                           rdfs:comment "This class refers to a non fictional human or non-human character in a narrative work of art."@en .


###  http://www.semanticweb.org/ontologies/2021/1/content#NonFictionalPlot
cont:NonFictionalPlot rdf:type owl:Class ;
                      rdfs:subClassOf cont:Plot ;
                      rdfs:comment "Plot based on truth and accuracy regarding information, events, or people."@en .


###  http://www.semanticweb.org/ontologies/2021/1/content#Opposing
cont:Opposing rdf:type owl:Class ;
              rdfs:subClassOf cont:CharacterStatus ;
              rdfs:comment "This class refers to a character in a narrative that is focused on by the primary storyline and in opposition to the leading character."@en .


###  http://www.semanticweb.org/ontologies/2021/1/content#Origin
cont:Origin rdf:type owl:Class ;
            rdfs:subClassOf cont:SociologicalCharacteristics ,
                            [ rdf:type owl:Restriction ;
                              owl:onProperty cont:isOriginOf ;
                              owl:allValuesFrom cont:Agent
                            ] ;
            owl:disjointWith cont:Profession ,
                             cont:SocialClass .


###  http://www.semanticweb.org/ontologies/2021/1/content#Person
cont:Person rdf:type owl:Class ;
            rdfs:subClassOf cont:Agent ;
            rdfs:comment "This class refers to a human being regarded as individuals."@en .


###  http://www.semanticweb.org/ontologies/2021/1/content#Plot
cont:Plot rdf:type owl:Class ;
          rdfs:comment "The main events of a play, novel, film, or similar work, devised and presented by the writer as an interrelated sequence."@en .


###  http://www.semanticweb.org/ontologies/2021/1/content#Poor
cont:Poor rdf:type owl:Class ;
          rdfs:subClassOf cont:EconomicStatus ;
          rdfs:comment "This class represents an economic status of an agent that lacks sufficient money to live at a standard considered comfortable by society."@en .


###  http://www.semanticweb.org/ontologies/2021/1/content#Profession
cont:Profession rdf:type owl:Class ;
                owl:equivalentClass <https://w3id.org/arco/ontology/context-description/Profession> ;
                rdfs:subClassOf cont:SociologicalCharacteristics ,
                                [ rdf:type owl:Restriction ;
                                  owl:onProperty cont:isProfessionOf ;
                                  owl:allValuesFrom cont:Agent
                                ] ;
                owl:disjointWith cont:SocialClass ;
                rdfs:comment "This class refers to the profession or occupation employed by an agent."@en .


###  http://www.semanticweb.org/ontologies/2021/1/content#Protagonist
cont:Protagonist rdf:type owl:Class ;
                 rdfs:subClassOf cont:CharacterRole ,
                                 [ rdf:type owl:Restriction ;
                                   owl:onProperty cont:hasCharacterStatus ;
                                   owl:allValuesFrom cont:Leading
                                 ] ;
                 rdfs:comment "This class refers to the main character of a creative work."@en .


###  http://www.semanticweb.org/ontologies/2021/1/content#Rich
cont:Rich rdf:type owl:Class ;
          rdfs:subClassOf cont:EconomicStatus ;
          rdfs:comment "This class represents an economic status of an agent that has a great deal of money or assets."@en .


###  http://www.semanticweb.org/ontologies/2021/1/content#Scenario
cont:Scenario rdf:type owl:Class ;
              rdfs:subClassOf cont:CulturalProduct ;
              rdfs:comment "A written outline of a film, novel, or stage work giving details of the plot and individual scenes."@en .


###  http://www.semanticweb.org/ontologies/2021/1/content#Screenwriter
cont:Screenwriter rdf:type owl:Class ;
                  rdfs:subClassOf cont:Writer ;
                  rdfs:comment "This class refers to a writer who wrote the script for TV, films, radio, comics or games."@en .


###  http://www.semanticweb.org/ontologies/2021/1/content#Secondary
cont:Secondary rdf:type owl:Class ;
               rdfs:subClassOf cont:CharacterRole ,
                               [ rdf:type owl:Restriction ;
                                 owl:onProperty cont:hasCharacterStatus ;
                                 owl:allValuesFrom cont:Supporting
                               ] ;
               rdfs:comment "This class refers to a minor character necessary for the plot due to the key details he/she reveals."@en .


###  http://www.semanticweb.org/ontologies/2021/1/content#SelfGood
cont:SelfGood rdf:type owl:Class ;
              rdfs:subClassOf cont:CharacterScope ;
              rdfs:comment "This class refers to the character personal advantage intention."@en .


###  http://www.semanticweb.org/ontologies/2021/1/content#SocialClass
cont:SocialClass rdf:type owl:Class ;
                 rdfs:subClassOf cont:SociologicalCharacteristics ;
                 rdfs:comment "This class refers to a grouping of people identifying themselves as belonging to a specific social class within a society. The main social classes are the aristocracy, the clergy and the commoners."@en .


###  http://www.semanticweb.org/ontologies/2021/1/content#SocialOrigin
cont:SocialOrigin rdf:type owl:Class ;
                  rdfs:subClassOf cont:Origin ,
                                  [ rdf:type owl:Restriction ;
                                    owl:onProperty cont:isDefinedBy ;
                                    owl:maxQualifiedCardinality "1"^^xsd:nonNegativeInteger ;
                                    owl:onClass cont:EconomicStatus
                                  ] ,
                                  [ rdf:type owl:Restriction ;
                                    owl:onProperty cont:isDefinedBy ;
                                    owl:maxQualifiedCardinality "1"^^xsd:nonNegativeInteger ;
                                    owl:onClass cont:SocialClass
                                  ] ;
                  rdfs:comment "This class refers to the peculiar trait in the origin of an individual related to its social provenance from the point of view of the social status and the social class defining them at their birth."@en .


###  http://www.semanticweb.org/ontologies/2021/1/content#SociologicalCharacteristics
cont:SociologicalCharacteristics rdf:type owl:Class ;
                                 rdfs:comment "This class refers to characteristics and features able to describe an agent from a sociological point of view." .


###  http://www.semanticweb.org/ontologies/2021/1/content#SupernaturalBeing
cont:SupernaturalBeing rdf:type owl:Class ;
                       rdfs:subClassOf cont:Agent ;
                       rdfs:comment "This class refers to kind of being from religion, mythology or folklore."@en .


###  http://www.semanticweb.org/ontologies/2021/1/content#Supporting
cont:Supporting rdf:type owl:Class ;
                rdfs:subClassOf cont:CharacterStatus ;
                rdfs:comment "This class refers to a character in a narrative that is not focused on by the primary storyline."@en .


###  http://www.semanticweb.org/ontologies/2021/1/content#TvSerie
cont:TvSerie rdf:type owl:Class ;
             rdfs:subClassOf cont:Scenario ;
             rdfs:comment "A group of programs created or adapted for television broadcast with a common series title."@en .


###  http://www.semanticweb.org/ontologies/2021/1/content#UniversalBad
cont:UniversalBad rdf:type owl:Class ;
                  rdfs:subClassOf cont:CharacterScope ;
                  rdfs:comment "An action that is against the interest of the world, applicable to all cases (humans, animals, enviroment etc.)."@en .


###  http://www.semanticweb.org/ontologies/2021/1/content#UniversalGood
cont:UniversalGood rdf:type owl:Class ;
                   rdfs:subClassOf cont:CharacterScope ;
                   rdfs:comment "An action that is in the interest of the world, applicable to all cases (humans, animals, enviroment etc.)."@en .


###  http://www.semanticweb.org/ontologies/2021/1/content#Villain
cont:Villain rdf:type owl:Class ;
             rdfs:subClassOf cont:CharacterType ,
                             [ rdf:type owl:Restriction ;
                               owl:onProperty cont:hasCharacterStatus ;
                               owl:someValuesFrom cont:CharacterStatus
                             ] ,
                             [ rdf:type owl:Restriction ;
                               owl:onProperty cont:hasCharacterRole ;
                               owl:allValuesFrom [ rdf:type owl:Class ;
                                                   owl:unionOf ( cont:Antagonist
                                                                 cont:Protagonist
                                                               )
                                                 ]
                             ] ,
                             [ rdf:type owl:Restriction ;
                               owl:onProperty cont:hasCharacterScope ;
                               owl:allValuesFrom cont:UniversalBad
                             ] ;
             rdfs:comment "This class refers to a character whose evil actions or motives are important to the plot."@en .


###  http://www.semanticweb.org/ontologies/2021/1/content#Writer
cont:Writer rdf:type owl:Class ;
            rdfs:subClassOf cont:Person ;
            rdfs:comment "This class refers to person who uses written words to communicate ideas and to produce works of literature."@en .


###  https://w3id.org/arco/ontology/context-description/Profession

###  https://w3id.org/arco/ontology/denotative-description/Environment

###  https://w3id.org/italia/onto/l0/Agent

#################################################################
#    General axioms
#################################################################

[ rdf:type owl:AllDisjointClasses ;
  owl:members ( cont:Animal
                cont:Character
                cont:Person
                cont:SupernaturalBeing
              )
] .


[ rdf:type owl:AllDisjointClasses ;
  owl:members ( cont:EthnicOrigin
                cont:GeographicOrigin
                cont:SocialOrigin
              )
] .


[ rdf:type owl:AllDisjointClasses ;
  owl:members ( cont:Medium
                cont:Poor
                cont:Rich
              )
] .


###  Generated by the OWL API (version 4.5.9.2019-02-01T07:24:44Z) https://github.com/owlcs/owlapi
